byteback-core/src/main/java/byteback/core/context/soot/SootContext.java
@@ -39,7 +39,6 @@ public class SootContext {
 
 	private void configure() {
 		options().setPhaseOption("jb", "use-original-names:true");
-		options().set_output_format(Options.output_format_jimple);
 		options().set_whole_program(true);
 		scene().loadBasicClasses();
 		log.info("Soot context initialized successfully");
