byteback-core/src/main/java/byteback/core/converter/soottoboogie/method/procedure/DefinitionsCollector.java
@@ -2,7 +2,8 @@ package byteback.core.converter.soottoboogie.method.procedure;
 
 import byteback.core.representation.soot.body.SootBodies;
 import byteback.core.util.Lazy;
-import java.util.Collection;
+import java.util.List;
+import java.util.Set;
 import java.util.stream.Collectors;
 import soot.Body;
 import soot.Local;
@@ -15,6 +16,7 @@ import soot.toolkits.scalar.SimpleLocalUses;
 public class DefinitionsCollector {
 
 	private Lazy<LocalDefs> definitions;
+
 	private Lazy<LocalUses> uses;
 
 	public DefinitionsCollector() {
@@ -31,15 +33,15 @@ public class DefinitionsCollector {
 		return definitionsOf(local).size() == 1;
 	}
 
-	public Collection<Unit> definitionsOfAt(final Local local, final Unit unit) {
+	public List<Unit> definitionsOfAt(final Local local, final Unit unit) {
 		return definitions.get().getDefsOfAt(local, unit);
 	}
 
-	public Collection<Unit> definitionsOf(final Local local) {
+	public Set<Unit> definitionsOf(final Local local) {
 		return definitions.get().getDefsOf(local).stream().collect(Collectors.toSet());
 	}
 
-	public Collection<Unit> usesOf(final Local local) {
+	public Set<Unit> usesOf(final Local local) {
 		return definitions.get().getDefsOf(local).stream().flatMap((unit) -> {
 			return uses.get().getUsesOf(unit).stream().map((pair) -> pair.unit).collect(Collectors.toSet()).stream();
 		}).collect(Collectors.toSet());
