byteback-core/src/main/java/byteback/core/preprocessing/BodyAggregator.java
@@ -1,0 +1,149 @@
+package byteback.core.preprocessing;
+
+import java.util.HashSet;
+import java.util.Iterator;
+import java.util.Set;
+import java.util.Stack;
+import java.util.concurrent.atomic.AtomicBoolean;
+
+import byteback.core.converter.soottoboogie.method.procedure.DefinitionsCollector;
+import byteback.core.representation.soot.body.SootExpressionVisitor;
+import byteback.core.representation.soot.body.SootStatementVisitor;
+import soot.Body;
+import soot.Local;
+import soot.Unit;
+import soot.Value;
+import soot.ValueBox;
+import soot.grimp.Grimp;
+import soot.grimp.GrimpBody;
+import soot.jimple.ArrayRef;
+import soot.jimple.AssignStmt;
+import soot.jimple.InstanceFieldRef;
+import soot.jimple.StaticFieldRef;
+import soot.util.Chain;
+
+public class BodyAggregator {
+
+	final DefinitionsCollector defCollector;
+
+	public BodyAggregator() {
+		this.defCollector = new DefinitionsCollector();
+	}
+
+	public void removeUnusedLocals(final Body body) {
+		final Chain<Local> locals = body.getLocals();
+		final Iterator<Local> iterator = body.getLocals().snapshotIterator();
+
+		defCollector.collect(body);
+
+		while (iterator.hasNext()) {
+			final Local local = iterator.next();
+
+			if (defCollector.usesOf(local).size() == 0) {
+				locals.remove(local);
+			}
+		}
+	}
+
+	public boolean hasLoop(final Local local, final Unit unit) {
+		final Stack<Local> next = new Stack<>();
+		final HashSet<Local> visited = new HashSet<>();
+
+		next.push(local);
+
+		while (!next.isEmpty()) {
+			final Local current = next.pop();
+			final Set<Unit> uses = defCollector.usesOf(current);
+			visited.add(current);
+
+			for (Unit use : uses) {
+				final AtomicBoolean looping = new AtomicBoolean(false);
+
+				use.apply(new SootStatementVisitor<>() {
+
+					@Override
+					public void caseAssignStmt(final AssignStmt assignment) {
+						assignment.getLeftOp().apply(new SootExpressionVisitor<>() {
+
+							private void addNext(final Value value) {
+								if (!visited.contains(local)) {
+									next.push(local);
+								} else {
+									looping.set(true);
+								}
+							}
+
+							@Override
+							public void caseLocal(final Local local) {
+								addNext(local);
+							}
+
+							@Override
+							public void caseArrayRef(final ArrayRef reference) {
+								addNext(reference);
+							}
+
+							@Override
+							public void caseStaticFieldRef(final StaticFieldRef reference) {
+								addNext(reference);
+							}
+
+							@Override
+							public void caseInstanceFieldRef(final InstanceFieldRef reference) {
+								addNext(reference);
+							}
+
+						});
+					}
+
+				});
+
+				if (looping.get()) {
+					return true;
+				}
+			}
+		}
+
+		return false;
+	}
+
+	public GrimpBody transform(final Body source) {
+		final GrimpBody body = Grimp.v().newBody(source, "gb");
+		Iterator<Unit> iterator = body.getUnits().snapshotIterator();
+		defCollector.collect(source);
+
+		while (iterator.hasNext()) {
+			final Unit unit = iterator.next();
+
+			for (final ValueBox box : unit.getUseBoxes()) {
+				final Value value = box.getValue();
+
+				value.apply(new SootExpressionVisitor<>() {
+
+					@Override
+					public void caseLocal(final Local local) {
+						final Set<Unit> definitions = defCollector.definitionsOf(local);
+						final Set<Unit> uses = defCollector.usesOf(local);
+						if (definitions.size() == 1 && uses.size() == 1 && !hasLoop(local, unit)) {
+							definitions.iterator().next().apply(new SootStatementVisitor<>() {
+
+								@Override
+								public void caseAssignStmt(final AssignStmt assignment) {
+									body.getUnits().remove(definitions.iterator().next());
+									box.setValue(assignment.getRightOp());
+								}
+
+							});
+						}
+					}
+
+				});
+			}
+		}
+
+		removeUnusedLocals(body);
+
+		return body;
+	}
+
+}
