byteback-core/src/main/java/byteback/core/preprocessing/DependencyCollector.java
@@ -1,0 +1,26 @@
+package byteback.core.preprocessing;
+
+import byteback.core.util.MultiMap;
+import soot.Local;
+import soot.Unit;
+import soot.Value;
+import soot.ValueBox;
+import soot.jimple.toolkits.infoflow.CachedEquivalentValue;
+import soot.util.Chain;
+
+public class DependencyCollector {
+
+	final MultiMap<Value, Unit> from;
+
+	final MultiMap<Unit, Value> to;
+
+	public DependencyCollector() {
+		this.from = new MultiMap<>();
+		this.to = new MultiMap<>();
+	}
+
+	public void collect(final Unit unit) {
+		Local local = null;
+	}
+
+}
